Factor out expr/stmt costs into MetricCosts.v
Also update bedrock2 semantics for new metrics, which fixes
FlattenExpr.v. All the other pipeline stages are now broken and need to
be patched.

bedrock2/src/bedrock2/MetricWeakestPrecondition.v
@@ -2,6 +2,7 @@ Require Import coqutil.Macros.subst coqutil.Macros.unique coqutil.Map.Interface 
 Require Import Coq.ZArith.BinIntDef coqutil.Word.Interface coqutil.Word.Bitwidth.
 Require Import coqutil.dlet bedrock2.Syntax bedrock2.Semantics.
 Require Import bedrock2.MetricLogging.
+Require Import bedrock2.MetricCosts.
 Require Import bedrock2.MetricSemantics.
 
 Section WeakestPrecondition.
@@ -11,13 +12,15 @@ Section WeakestPrecondition.
   Implicit Types (t : trace) (m : mem) (l : locals).
 
   Local Notation metrics := MetricLog.
-  
+  Local Notation UNK := String.EmptyString.
+
+  (* TODO XXX address inconsistency in where metrics are added *)
   Definition literal v mc (post : (word * metrics) -> Prop) : Prop :=
-    dlet! v := word.of_Z v in post (v, addMetricInstructions 8 (addMetricLoads 8 mc)).
+    dlet! v := word.of_Z v in post (v, cost_lit isRegStr UNK mc).
   Definition get (l : locals) (x : String.string) mc (post : (word * metrics) -> Prop) : Prop :=
-    exists v, map.get l x = Some v /\ post (v, addMetricInstructions 1 (addMetricLoads 2 mc)).
+    exists v, map.get l x = Some v /\ post (v, cost_set isRegStr UNK x mc).
   Definition load s m a mc (post: (word * metrics) -> Prop) : Prop :=
-    exists v, load s m a = Some v /\ post(v, addMetricInstructions 1 (addMetricLoads 2 mc)).
+    exists v, load s m a = Some v /\ post (v, mc).
   Definition store sz m a v post :=
     exists m', store sz m a v = Some m' /\ post m'.
 
@@ -32,17 +35,15 @@ Section WeakestPrecondition.
       | expr.op op e1 e2 =>
         rec e1 mc (fun '(v1, mc') =>
         rec e2 mc' (fun '(v2, mc'') =>
-        post (interp_binop op v1 v2, addMetricInstructions 2 (addMetricLoads 2 mc''))))
+        post (interp_binop op v1 v2, cost_op isRegStr UNK UNK UNK mc'')))
       | expr.load s e =>
        rec e mc (fun '(a, mc') =>
-        load s m a mc' post)
+        load s m a (cost_load isRegStr UNK UNK mc') post)
       | expr.inlinetable s t e =>
          rec e mc (fun '(a, mc') =>
-        load s (map.of_list_word t) a (addMetricInstructions 2
-                                      (addMetricLoads 2
-                                      (addMetricJumps 1 mc'))) post)
+        load s (map.of_list_word t) a (cost_inlinetable isRegStr UNK UNK mc') post)
       | expr.ite c e1 e2 =>
-        rec c mc (fun '(b, mc') => rec (if word.eqb b (word.of_Z 0) then e2 else e1) (addMetricInstructions 2 (addMetricLoads 2 (addMetricJumps 1 mc'))) post) 
+        rec c mc (fun '(b, mc') => rec (if word.eqb b (word.of_Z 0) then e2 else e1) (cost_if isRegStr UNK (Some UNK) mc') post)
     end.
     Fixpoint expr e := expr_body expr e.
   End WithMemAndLocals.
@@ -77,7 +78,7 @@ Section WeakestPrecondition.
       | cmd.set x ev =>
           exists v mc', dexpr m l ev mc (v, mc') /\
           dlet! l := map.put l x v in
-          post t m l (addMetricInstructions 1 (addMetricLoads 1 mc'))
+          post t m l (cost_set isRegStr x UNK mc')
       | cmd.unset x =>
         dlet! l := map.remove l x in
             post t m l mc
@@ -85,43 +86,41 @@ Section WeakestPrecondition.
        exists a mc', dexpr m l ea mc (a, mc') /\
        exists v mc'', dexpr m l ev mc (v, mc'') /\
        store sz m a v (fun m =>
-       post t m l (addMetricInstructions 1 (addMetricLoads 1 (addMetricStores 1 mc''))))
+       post t m l (cost_store isRegStr UNK UNK mc''))
       | cmd.stackalloc x n c =>
         Z.modulo n (bytes_per_word width) = 0 /\
         forall a mStack mCombined,
           anybytes a n mStack -> map.split mCombined m mStack ->
           dlet! l := map.put l x a in
-          rec c t mCombined l (addMetricInstructions 1 (addMetricLoads 1 mc))
+          rec c t mCombined l (cost_stackalloc isRegStr x mc)
           (fun t' mCombined' l' mc' =>
           exists m' mStack',
           anybytes a n mStack' /\ map.split mCombined' m' mStack' /\
           post t' m' l' mc')
-     | cmd.cond br ct cf =>     
+     | cmd.cond br ct cf =>
         exists v mc', dexpr m l br mc (v, mc') /\
-        dlet! mc'' := addMetricInstructions 2 (addMetricLoads 2 (addMetricJumps 1 mc')) in
+        dlet! mc'' := cost_if isRegStr UNK (Some UNK) mc' in
         (word.unsigned v <> 0%Z -> rec ct t m l mc'' post) /\
-        (word.unsigned v = 0%Z -> rec cf t m l mc'' post)                    
+        (word.unsigned v = 0%Z -> rec cf t m l mc'' post)
     | cmd.seq c1 c2 =>
         rec c1 t m l mc (fun t m l mc => rec c2 t m l mc post)
     | cmd.while _ _ => MetricSemantics.exec e c t m l mc post
     | cmd.call binds fname arges =>
         exists args mc', dexprs m l arges mc (args, mc') /\
         MetricSemantics.call e fname t m args mc (fun t m rets mc'' =>
-        exists l', map.putmany_of_list_zip binds rets l = Some l' /\ post t m l' (addMetricInstructions 100 (addMetricJumps 100 (addMetricLoads 100 (addMetricStores 100 mc'')))))
+        exists l', map.putmany_of_list_zip binds rets l = Some l' /\ post t m l' (cost_call_internal PreSpill mc''))
     | cmd.interact binds action arges =>
-        exists args mc', dexprs m l arges mc (args, mc') /\                   
+        exists args mc', dexprs m l arges mc (args, mc') /\
         exists mKeep mGive, map.split m mKeep mGive /\
         ext_spec t mGive action args (fun mReceive rets =>
           exists l', map.putmany_of_list_zip binds rets l = Some l' /\
           forall m', map.split m' mKeep mReceive ->
-          post (cons ((mGive, action, args), (mReceive, rets)) t) m' l' (addMetricInstructions 1
-                                                                        (addMetricStores 1
-                                                                        (addMetricLoads 2 mc'))))
+          post (cons ((mGive, action, args), (mReceive, rets)) t) m' l' (cost_interact PreSpill mc'))
       end.
 
     Fixpoint cmd c := cmd_body cmd c.
   End WithFunctions.
-  
+
   Definition func call '(innames, outnames, c) (t : trace) (m : mem) (args : list word) (mc : metrics) (post : trace -> mem -> list word -> metrics -> Prop) :=
 exists l, map.of_list_zip innames args = Some l /\
       cmd call c t m l mc (fun t m l mc =>
