bedrock2/src/bedrock2/MetricCosts.v
@@ -1,0 +1,175 @@
+Require Import BinIntDef.
+Require Import Coq.Strings.String.
+Require Import bedrock2.MetricLogging.
+From coqutil.Tactics Require Import destr.
+
+Local Open Scope MetricH_scope.
+
+Inductive compphase: Type :=
+| PreSpill
+| PostSpill.
+
+Section FlatImpExec.
+
+  Context {varname: Type}.
+  Variable (phase: compphase).
+  Variable (isReg: varname -> bool).
+
+  Definition cost_interact mc :=
+    match phase with
+    | PreSpill => (addMetricInstructions 100 (addMetricJumps 100 (addMetricStores 100 (addMetricLoads 100 mc))))
+    | PostSpill => (addMetricInstructions 50 (addMetricJumps 50 (addMetricStores 50 (addMetricLoads 50 mc))))
+    end.
+
+  Definition cost_call_internal mc :=
+    match phase with
+    | PreSpill => addMetricInstructions 100 (addMetricJumps 100 (addMetricLoads 100 (addMetricStores 100 mc)))
+    | PostSpill => addMetricInstructions 50 (addMetricJumps 50 (addMetricLoads 50 (addMetricStores 50 mc)))
+    end.
+
+  Definition cost_call_external mc :=
+    match phase with
+    | PreSpill => addMetricInstructions 100 (addMetricJumps 100 (addMetricLoads 100 (addMetricStores 100 mc)))
+    | PostSpill => addMetricInstructions 50 (addMetricJumps 50 (addMetricLoads 50 (addMetricStores 50 mc)))
+    end.
+
+  (* TODO think about a non-fixed bound on the cost of function preamble and postamble *)
+
+  Definition cost_load x a mc :=
+    match (isReg x, isReg a) with
+    | (false, false) => (addMetricInstructions 3 (addMetricLoads 5 (addMetricStores 1 mc)))
+    | (false,  true) => (addMetricInstructions 2 (addMetricLoads 3 (addMetricStores 1 mc)))
+    | ( true, false) => (addMetricInstructions 2 (addMetricLoads 4 mc))
+    | ( true,  true) => (addMetricInstructions 1 (addMetricLoads 2 mc))
+    end.
+
+  Definition cost_store a v mc :=
+    match (isReg a, isReg v) with
+    | (false, false) => (addMetricInstructions 3 (addMetricLoads 5 (addMetricStores 1 mc)))
+    | (false,  true) => (addMetricInstructions 2 (addMetricLoads 3 (addMetricStores 1 mc)))
+    | ( true, false) => (addMetricInstructions 2 (addMetricLoads 3 (addMetricStores 1 mc)))
+    | ( true,  true) => (addMetricInstructions 1 (addMetricLoads 1 (addMetricStores 1 mc)))
+    end.
+
+  Definition cost_inlinetable x i mc :=
+    match (isReg x, isReg i) with
+    | (false, false) => (addMetricInstructions 5 (addMetricLoads 7 (addMetricStores 1 (addMetricJumps 1 mc))))
+    | (false,  true) => (addMetricInstructions 4 (addMetricLoads 5 (addMetricStores 1 (addMetricJumps 1 mc))))
+    | ( true, false) => (addMetricInstructions 4 (addMetricLoads 6 (addMetricJumps 1 mc)))
+    | ( true,  true) => (addMetricInstructions 3 (addMetricLoads 4 (addMetricJumps 1 mc)))
+    end.
+
+  Definition cost_stackalloc x mc :=
+    match isReg x with
+    | false => (addMetricInstructions 2 (addMetricLoads 2 (addMetricStores 1 mc)))
+    |  true => (addMetricInstructions 1 (addMetricLoads 1 mc))
+    end.
+
+  Definition cost_lit x mc :=
+    match isReg x with
+    | false => (addMetricInstructions 9 (addMetricLoads 9 (addMetricStores 1 mc)))
+    |  true => (addMetricInstructions 8 (addMetricLoads 8 mc))
+    end.
+
+  Definition cost_op x y z mc :=
+    match (isReg x, isReg y, isReg z) with
+    | (false, false, false) => (addMetricInstructions 5 (addMetricLoads 7 (addMetricStores 1 mc)))
+    | (false, false,  true) | (false,  true, false) => (addMetricInstructions 4 (addMetricLoads 5 (addMetricStores 1 mc)))
+    | (false,  true,  true) => (addMetricInstructions 3 (addMetricLoads 3 (addMetricStores 1 mc)))
+    | ( true, false, false) => (addMetricInstructions 4 (addMetricLoads 6 mc))
+    | ( true, false,  true) | ( true,  true, false) => (addMetricInstructions 3 (addMetricLoads 4 mc))
+    | ( true,  true,  true) => (addMetricInstructions 2 (addMetricLoads 2 mc))
+    end.
+
+  Definition cost_set x y mc :=
+    match (isReg x, isReg y) with
+    | (false, false) => (addMetricInstructions 3 (addMetricLoads 4 (addMetricStores 1 mc)))
+    | (false,  true) => (addMetricInstructions 2 (addMetricLoads 2 (addMetricStores 1 mc)))
+    | ( true, false) => (addMetricInstructions 2 (addMetricLoads 3 mc))
+    | ( true,  true) => (addMetricInstructions 1 (addMetricLoads 1 mc))
+    end.
+
+    Definition cost_if x y mc :=
+      match (isReg x, match y with | Some y' => isReg y' | None => true end) with
+      | (false, false) => (addMetricInstructions 4 (addMetricLoads 6 (addMetricJumps 1 mc)))
+      | (false,  true) | ( true, false) => (addMetricInstructions 3 (addMetricLoads 4 (addMetricJumps 1 mc)))
+      | ( true,  true) => (addMetricInstructions 2 (addMetricLoads 2 (addMetricJumps 1 mc)))
+      end.
+
+    Definition cost_loop_true x y mc :=
+      match (isReg x, match y with | Some y' => isReg y' | None => true end) with
+      | (false, false) => (addMetricInstructions 4 (addMetricLoads 6 (addMetricJumps 1 mc)))
+      | (false,  true) | ( true, false) => (addMetricInstructions 3 (addMetricLoads 4 (addMetricJumps 1 mc)))
+      | ( true,  true) => (addMetricInstructions 2 (addMetricLoads 2 (addMetricJumps 1 mc)))
+      end.
+
+    Definition cost_loop_false x y mc :=
+      match (isReg x, match y with | Some y' => isReg y' | None => true end) with
+      | (false, false) => (addMetricInstructions 3 (addMetricLoads 5 (addMetricJumps 1 mc)))
+      | (false,  true) | ( true, false) => (addMetricInstructions 2 (addMetricLoads 3 (addMetricJumps 1 mc)))
+      | ( true,  true) => (addMetricInstructions 1 (addMetricLoads 1 (addMetricJumps 1 mc)))
+      end.
+
+End FlatImpExec.
+
+Definition isRegZ (var : Z) : bool :=
+  Z.leb var 31.
+
+Definition isRegStr (var : String.string) : bool :=
+  String.prefix "reg_" var.
+
+Ltac cost_unfold :=
+  unfold cost_interact, cost_call_internal, cost_call_external, cost_load,
+  cost_store, cost_inlinetable, cost_stackalloc, cost_lit, cost_op, cost_set,
+  cost_if, cost_loop_true, cost_loop_false in *.
+
+Ltac cost_destr :=
+  repeat match goal with
+         | x : compphase |- _ => destr x
+         | _ : context[if ?x then _ else _] |- _ => destr x; try discriminate
+         | |- context[if ?x then _ else _] => destr x; try discriminate
+         end; unfold EmptyMetricLog.
+
+Ltac cost_solve := cost_unfold; cost_destr; try solve_MetricLog.
+Ltac cost_solve_piecewise := cost_unfold; cost_destr; try solve_MetricLog_piecewise.
+
+Definition metrics_additive f := forall mc, f mc - mc = f EmptyMetricLog.
+#[global] Transparent metrics_additive.
+
+Ltac t := unfold metrics_additive; intros; cost_solve_piecewise.
+Lemma cost_additive_interact : forall phase, metrics_additive (cost_interact phase). Proof. t. Qed.
+Lemma cost_additive_call_internal : forall phase, metrics_additive (cost_call_internal phase). Proof. t. Qed.
+Lemma cost_additive_call_external : forall phase, metrics_additive (cost_call_external phase). Proof. t. Qed.
+Lemma cost_additive_load : forall varname isReg x a, metrics_additive (@cost_load varname isReg x a). Proof. t. Qed.
+Lemma cost_additive_store : forall varname isReg x a, metrics_additive (@cost_store varname isReg x a). Proof. t. Qed.
+Lemma cost_additive_inlinetable : forall varname isReg x a, metrics_additive (@cost_inlinetable varname isReg x a). Proof. t. Qed.
+Lemma cost_additive_stackalloc : forall varname isReg x, metrics_additive (@cost_stackalloc varname isReg x). Proof. t. Qed.
+Lemma cost_additive_lit : forall varname isReg x, metrics_additive (@cost_lit varname isReg x). Proof. t. Qed.
+Lemma cost_additive_op : forall varname isReg x y z, metrics_additive (@cost_op varname isReg x y z). Proof. t. Qed.
+Lemma cost_additive_set : forall varname isReg x y, metrics_additive (@cost_set varname isReg x y). Proof. t. Qed.
+Lemma cost_additive_if : forall varname isReg x y, metrics_additive (@cost_if varname isReg x y). Proof. t. Qed.
+Lemma cost_additive_loop_true : forall varname isReg x y, metrics_additive (@cost_loop_true varname isReg x y). Proof. t. Qed.
+Lemma cost_additive_loop_false : forall varname isReg x y, metrics_additive (@cost_loop_false varname isReg x y). Proof. t. Qed.
+
+(* COQBUG:
+   these cannot have "in *", because this causes a crash if the environment contains a Semantics.ExtSpec.
+     Anomaly "Unable to handle arbitrary u+k <= v constraints."
+     Please report at http://coq.inria.fr/bugs/.
+   to use these in hypotheses, revert them first *)
+Ltac cost_additive := repeat (
+  rewrite cost_additive_interact ||
+  rewrite cost_additive_call_internal ||
+  rewrite cost_additive_call_external ||
+  rewrite cost_additive_load ||
+  rewrite cost_additive_store ||
+  rewrite cost_additive_inlinetable ||
+  rewrite cost_additive_stackalloc ||
+  rewrite cost_additive_lit ||
+  rewrite cost_additive_op ||
+  rewrite cost_additive_set ||
+  rewrite cost_additive_if ||
+  rewrite cost_additive_loop_true ||
+  rewrite cost_additive_loop_false
+  ).
+
+Ltac cost_hammer := cost_additive; try solve [eauto 3 with metric_arith | cost_solve].
